\documentclass[a4paper]{amsart}

\usepackage{amsmath}
\newtheorem{theorem}{Satz}[section]
\newtheorem{corollary}{Korollar}[theorem]
\newtheorem{lemma}[theorem]{Lemma}
\usepackage{hyperref}

\usepackage{tensor}

\begin{document}


Further simplification:
\begin{align*}
(T_{\mathring{\mathcal{L}}})^{\mu \nu} 
&= 
- \frac{1}{8}
\Bigl(  
3 (\partial_\lambda 
\tensor{e}{^c_\kappa}) 
+
(\partial_\kappa \tensor{e}{^c_\lambda})  
\Bigr) 
\,
\tensor{e}{_c^\kappa} 
\, 
\bar{\psi} \, 
( g^{\lambda\mu}\gamma^\nu 
+ g^{\lambda\nu}\gamma^\mu )
\psi
\nonumber \\ %=========================
&\qquad 
+
\frac{1}{2} 
g^{\mu\nu} 
[ 
(\partial_\lambda \tensor{e}{^c_\kappa})
+
(\partial_\kappa \tensor{e}{^c_\lambda}) 
]  
\tensor{e}{_c^\kappa} 
\, 
\bar{\psi} 
\, 
\gamma^\lambda  
\psi
\nonumber \\ %======================
&\qquad 
+ 
\frac{i}{4} 
\bar{\psi} \,
\Bigl[  
-
\tensor{e}{_c_\rho}
[
(\partial_\lambda \tensor{e}{^c_\kappa})
-  
(\partial_\kappa \tensor{e}{^c_\lambda})
]
(  
g^{\kappa \nu}
\sigma^{\mu\lambda}
+ 
g^{\kappa \mu}
\sigma^{\nu\lambda}
) 
\gamma^\rho  
- 
(\partial_\lambda\tensor{e}{^c_\kappa})
\sigma^{\lambda\kappa}
(
\tensor{e}{_c^\mu}
\gamma^\nu
+
\tensor{e}{_c^\nu}
\gamma^\mu
)
\Bigr]
\psi
%==========================
\nonumber \\ 
&\qquad 
- \frac{1}{2}  g^{\mu\nu}
\Bigl[ 
(\partial_\lambda\bar{\psi}) 
\, \gamma^\lambda \, \psi 
+ \bar{\psi} \,\gamma^\lambda 
\, (\partial_\lambda \psi)
\Bigr]
+
\frac{1}{4}  
(\partial_\lambda\bar{\psi}) \,
( g^{\lambda\mu}\gamma^\nu 
+ g^{\lambda\nu}\gamma^\mu )
\, 
\psi 
+
\frac{1}{4} \bar{\psi} \,
( g^{\lambda\mu}\gamma^\nu 
+ g^{\lambda\nu}\gamma^\mu )
\, 
(\partial_\lambda \psi)
\end{align*}


\end{document}
